James C - decided against chapter 13, 14, started 15

isabelle/Chapter15_2_Typechecking.thy
@@ -1,13 +1,13 @@
-theory Chapter14_3_Typechecking
-imports Chapter14_2_Expressions
+theory Chapter15_2_Typechecking
+imports Chapter15_1_Language
 begin
 
 inductive typecheck :: "type env => expr => type => bool"
 where tc_var [simp]: "lookup gam x = Some t ==> typecheck gam (Var x) t"
     | tc_zero [simp]: "typecheck gam Zero Nat"
     | tc_suc [simp]: "typecheck gam e Nat ==> typecheck gam (Suc e) Nat"
-    | tc_natrec [simp]: "typecheck gam et Nat ==> typecheck gam e0 t ==> 
-                typecheck (extend (extend gam t) Nat) es t ==> typecheck gam (NatRec et e0 es) t"
+    | tc_rec [simp]: "typecheck gam et Nat ==> typecheck gam e0 t ==> 
+                typecheck (extend (extend gam t) Nat) es t ==> typecheck gam (Rec et e0 es) t"
     | tc_lam [simp]: "typecheck (extend gam t1) e t2 ==> typecheck gam (Lam t1 e) (Arrow t1 t2)"
     | tc_appl [simp]: "typecheck gam e1 (Arrow t2 t) ==> typecheck gam e2 t2 ==> 
                 typecheck gam (Appl e1 e2) t"
@@ -21,18 +21,11 @@ where tc_var [simp]: "lookup gam x = Some t ==> typecheck gam (Var x) t"
                 typecheck (extend gam t2) er t ==> typecheck gam (Case et el er) t"
     | tc_inl [simp]: "typecheck gam e t1 ==> typecheck gam (InL t1 t2 e) (Sum t1 t2)"
     | tc_inr [simp]: "typecheck gam e t2 ==> typecheck gam (InR t1 t2 e) (Sum t1 t2)"
-    | tc_fold [simp]: "typecheck gam e (type_subst (Ind t) t) ==> typecheck gam (Fold t e) (Ind t)"
-    | tc_rec [simp]: "typecheck (extend gam (type_subst t' t)) e1 t' ==> 
-                typecheck gam e2 (ind t) ==> typecheck gam (Rec t e1 e2) t'"
-    | tc_unfold [simp]: "typecheck gam e (Coind t) ==> 
-                typecheck gam (Unfold t e) (type_subst (Coind t) t)"
-    | tc_gen [simp]: "typecheck gam e2 t2 ==> typecheck (extend gam t2) e1 (type_subst t2 t) ==> 
-                typecheck gam (Gen t e1 e2) (Coind t)"
 
 inductive_cases [elim!]: "typecheck gam (Var x) t"
 inductive_cases [elim!]: "typecheck gam Zero t"
 inductive_cases [elim!]: "typecheck gam (Suc e) t"
-inductive_cases [elim!]: "typecheck gam (NatRec et e0 es) t"
+inductive_cases [elim!]: "typecheck gam (Rec et e0 es) t"
 inductive_cases [elim!]: "typecheck gam (Lam t1 e) t"
 inductive_cases [elim!]: "typecheck gam (Appl e1 e2) t"
 inductive_cases [elim!]: "typecheck gam Triv t"
@@ -43,10 +36,6 @@ inductive_cases [elim!]: "typecheck gam (Abort t1 e) t"
 inductive_cases [elim!]: "typecheck gam (Case et el er) t"
 inductive_cases [elim!]: "typecheck gam (InL t1 t2 e) t"
 inductive_cases [elim!]: "typecheck gam (InR t1 t2 e) t"
-inductive_cases [elim!]: "typecheck gam (Fold t1 e) t"
-inductive_cases [elim!]: "typecheck gam (Rec t1 e1 e2) t"
-inductive_cases [elim!]: "typecheck gam (Unfold t1 e) t"
-inductive_cases [elim!]: "typecheck gam (Gen t1 e1 e2) t"
 
 lemma [simp]: "typecheck gam e t ==> n in gam ==> 
          typecheck (extend_at n gam t') (insert n e) t"
