isabelle/Chapter15_3_Evaluation.thy
@@ -1,12 +1,12 @@
-theory Chapter13_4_Evaluation
-imports Chapter13_3_Typechecking
+theory Chapter15_3_Evaluation
+imports Chapter15_2_Typechecking
 begin
 
 primrec is_val :: "expr => bool"
 where "is_val (Var v) = False"
     | "is_val Zero = True"
     | "is_val (Suc e) = is_val e"
-    | "is_val (NatRec et e0 es) = False"
+    | "is_val (Rec et e0 es) = False"
     | "is_val (Lam t e) = True"
     | "is_val (Appl e1 e2) = False"
     | "is_val Triv = True"
@@ -17,14 +17,13 @@ where "is_val (Var v) = False"
     | "is_val (Case et el er) = False"
     | "is_val (InL t1 t2 e) = is_val e"
     | "is_val (InR t1 t2 e) = is_val e"
-    | "is_val (Map t e1 e2) = False"
 
 inductive eval :: "expr => expr => bool"
 where eval_suc [simp]: "eval e e' ==> eval (Suc e) (Suc e')"
-    | eval_natrec_1 [simp]: "eval et et' ==> eval (NatRec et e0 es) (NatRec et e0 es)"
-    | eval_natrec_2 [simp]: "eval (NatRec Zero e0 es) e0"
-    | eval_natrec_3 [simp]: "is_val et ==> 
-            eval (NatRec (Suc et) e0 es) (subst (NatRec et e0 es) (subst et es))"
+    | eval_rec_1 [simp]: "eval et et' ==> eval (Rec et e0 es) (Rec et e0 es)"
+    | eval_rec_2 [simp]: "eval (Rec Zero e0 es) e0"
+    | eval_rec_3 [simp]: "is_val et ==> 
+            eval (Rec (Suc et) e0 es) (subst (Rec et e0 es) (subst et es))"
     | eval_appl_1 [simp]: "eval e1 e1' ==> eval (Appl e1 e2) (Appl e1' e2)"
     | eval_appl_2 [simp]: "is_val e1 ==> eval e2 e2' ==> eval (Appl e1 e2) (Appl e1 e2')"
     | eval_appl_3 [simp]: "is_val e2 ==> eval (Appl (Lam t2 e1) e2) (subst e2 e1)"
@@ -71,13 +70,13 @@ theorem preservation: "eval e e' ==> typecheck gam e t ==> typecheck gam e' t"
 proof (induction e e' arbitrary: t rule: eval.induct)
 case eval_suc 
   thus ?case by fastforce
-next case eval_natrec_1 
+next case eval_rec_1 
   thus ?case by fastforce
-next case eval_natrec_2 
+next case eval_rec_2 
   thus ?case by fastforce
-next case (eval_natrec_3 et e0 es)
-  from eval_natrec_3 canonical_nat_no_vars have "typecheck (extend gam t) (subst et es) t" by auto
-  with eval_natrec_3 show ?case by fastforce
+next case (eval_rec_3 et e0 es)
+  from eval_rec_3 canonical_nat_no_vars have "typecheck (extend gam t) (subst et es) t" by auto
+  with eval_rec_3 show ?case by fastforce
 next case eval_appl_1 
   thus ?case by fastforce
 next case eval_appl_2 
@@ -118,8 +117,8 @@ next case tc_zero
   thus ?case by simp
 next case tc_suc
   thus ?case by (metis eval_suc is_val.simps(3))
-next case tc_natrec
-  thus ?case by (metis eval_natrec_1 eval_natrec_2 eval_natrec_3 is_val.simps(3) canonical_nat)
+next case tc_rec
+  thus ?case by (metis eval_rec_1 eval_rec_2 eval_rec_3 is_val.simps(3) canonical_nat)
 next case tc_lam
   thus ?case by simp
 next case tc_appl
@@ -141,8 +140,6 @@ next case tc_inl
   thus ?case by (metis eval_inl is_val.simps(13))
 next case tc_inr
   thus ?case by (metis eval_inr is_val.simps(14))
-next case tc_map
-  thus ?case try
 qed
 
 end
