isabelle/Chapter15_1_Language.thy
@@ -1,12 +1,20 @@
-theory Chapter13_2_Expressions
-imports Chapter13_1_Types
+theory Chapter15_1_Language
+imports DeBruijnEnvironment
 begin
+
+datatype type = 
+  Nat
+| Arrow type type
+| Unit
+| Prod type type
+| Void
+| Sum type type
 
 datatype expr = 
   Var var
 | Zero
 | Suc expr
-| NatRec expr expr expr
+| Rec expr expr expr
 | Lam type expr
 | Appl expr expr
 | Triv
@@ -17,13 +25,12 @@ datatype expr =
 | Case expr expr expr
 | InL type type expr
 | InR type type expr
-| Map type expr expr
 
 primrec insert :: "var => expr => expr"
 where "insert n (Var v) = Var (incr n v)"
     | "insert n Zero = Zero"
     | "insert n (Suc e) = Suc (insert n e)"
-    | "insert n (NatRec et e0 es) = NatRec (insert n et) (insert n e0) (insert (next (next n)) es)"
+    | "insert n (Rec et e0 es) = Rec (insert n et) (insert n e0) (insert (next (next n)) es)"
     | "insert n (Lam t e) = Lam t (insert (next n) e)"
     | "insert n (Appl e1 e2) = Appl (insert n e1) (insert n e2)"
     | "insert n Triv = Triv"
@@ -34,13 +41,12 @@ where "insert n (Var v) = Var (incr n v)"
     | "insert n (Case et el er) = Case (insert n et) (insert (next n) el) (insert (next n) er)"
     | "insert n (InL t1 t2 e) = InL t1 t2 (insert n e)"
     | "insert n (InR t1 t2 e) = InR t1 t2 (insert n e)"
-    | "insert n (Map t e1 e2) = Map t (insert (next n) e1) (insert n e2)"
 
 primrec remove :: "var => expr => expr"
 where "remove n (Var v) = Var (subr n v)"
     | "remove n Zero = Zero"
     | "remove n (Suc e) = Suc (remove n e)"
-    | "remove n (NatRec et e0 es) = NatRec (remove n et) (remove n e0) (remove (next (next n)) es)"
+    | "remove n (Rec et e0 es) = Rec (remove n et) (remove n e0) (remove (next (next n)) es)"
     | "remove n (Lam t e) = Lam t (remove (next n) e)"
     | "remove n (Appl e1 e2) = Appl (remove n e1) (remove n e2)"
     | "remove n Triv = Triv"
@@ -51,14 +57,13 @@ where "remove n (Var v) = Var (subr n v)"
     | "remove n (Case et el er) = Case (remove n et) (remove (next n) el) (remove (next n) er)"
     | "remove n (InL t1 t2 e) = InL t1 t2 (remove n e)"
     | "remove n (InR t1 t2 e) = InR t1 t2 (remove n e)"
-    | "remove n (Map t e1 e2) = Map t (remove (next n) e1) (remove n e2)"
 
 primrec subst' :: "var => expr => expr => expr"
 where "subst' n e' (Var v) = (if v = n then e' else Var v)"
     | "subst' n e' Zero = Zero"
     | "subst' n e' (Suc e) = Suc (subst' n e' e)"
-    | "subst' n e' (NatRec et e0 es) = 
-                      NatRec (subst' n e' et) 
+    | "subst' n e' (Rec et e0 es) = 
+                      Rec (subst' n e' et) 
                           (subst' n e' e0) 
                           (subst' (next (next n)) (insert first (insert first e')) es)"
     | "subst' n e' (Lam t e) = Lam t (subst' (next n) (insert first e') e)"
@@ -74,7 +79,6 @@ where "subst' n e' (Var v) = (if v = n then e' else Var v)"
                            (subst' (next n) (insert first e') er)"
     | "subst' n e' (InL t1 t2 e) = InL t1 t2 (subst' n e' e)"
     | "subst' n e' (InR t1 t2 e) = InR t1 t2 (subst' n e' e)"
-    | "subst' n e' (Map t e1 e2) = Map t (subst' (next n) (insert first e') e1) (subst' n e' e2)"
 
 definition subst :: "expr => expr => expr"
 where "subst e' e = remove first (subst' first (insert first e') e)"
